sepcomp/effect_simulations_lemmas.v
@@ -18,6 +18,7 @@ Require Import VST.sepcomp.structured_injections.
 Require Import VST.sepcomp.reach.
 Require Import VST.sepcomp.effect_simulations.
 
+(*
 Section Eff_INJ_SIMU_DIAGRAMS.
   Context {F1 V1 C1 F2 V2 C2:Type}
           {Sem1 : @EffectSem (Genv.t F1 V1) C1}
@@ -1201,3 +1202,4 @@ Proof. intros.
   remember (X b) as d.
   destruct d; trivial.
 Qed.
+*)
