veric/jstep.v
@@ -4,26 +4,26 @@ Require Import VST.concurrency.core_semantics.
 
 Module FSem.
 Record t M TM := mk {
-    F : forall G C, @CoreSemantics G C M -> @CoreSemantics G C TM
+    F : forall C, @CoreSemantics C M -> @CoreSemantics C TM
   ; E : TM -> M
   ; P : TM -> TM -> Prop
-  ; step  : forall G C sem ge c m c' m',
-            @corestep _ _ _ (F G C sem) ge c m c' m' =
-           (@corestep _ _ _ sem ge c (E m) c' (E m') /\ P m m')
-  ; init : forall G C sem n m v vl q,
-     initial_core (F G C sem) n m q v vl <->
+  ; step  : forall C sem c m c' m',
+            @corestep _ _ (F C sem) c m c' m' =
+           (@corestep _ _ sem c (E m) c' (E m') /\ P m m')
+  ; init : forall C sem n m v vl q,
+     initial_core (F C sem) n m q v vl <->
      initial_core sem n (E m) q v vl
-  ; atext  : forall G C sem c m,
-      at_external (F G C sem) c m = at_external sem c (E m)
-  ; aftext : forall G C sem ret c m,
-      after_external (F G C sem) ret c m = after_external sem ret c (E m)
-  ; halted : forall G C sem, halted (F G C sem) = halted sem
+  ; atext  : forall C sem c m,
+      at_external (F C sem) c m = at_external sem c (E m)
+  ; aftext : forall C sem ret c m,
+      after_external (F C sem) ret c m = after_external sem ret c (E m)
+  ; halted : forall C sem, halted (F C sem) = halted sem
   }.
 End FSem.
 
 Module IdFSem.
 Program Definition t M : FSem.t M M :=
-  FSem.mk M M (fun G C sem => sem) id (fun _ _ => True) _ _ _ _ _.
+  FSem.mk M M (fun C sem => sem) id (fun _ _ => True) _ _ _ _ _.
 Next Obligation.
 apply prop_ext.
 split; intros H.
